MPL/ProofMode/Tactics/WP.lean
@@ -33,8 +33,7 @@ open Lean Elab Tactic Meta
   specifications (which can be lossy) instead of information preserving rewrites.
 -/
 elab "mwp" : tactic => do
-  let mvar ← getMainGoal
-  let some _ := parseMGoal? (← instantiateMVars <| ← mvar.getType) | throwError "mwp: not in proof mode"
+  let (mvar, _) ← mStart (← getMainGoal)
   -- Somehow, conv in ... => rfl breaks the use of `withCollectingNewGoalsFrom` in `mspec`.
   -- I won't investigate because wp_simp will be replaced anyway.
   --  let (mvars, _) ← runTactic mvar (← `(tactic| conv in SPred.entails _ _ => arg 2; tactic => wp_simp))
