Test/Toy.lean
@@ -255,56 +255,53 @@ theorem fib_triple : ⦃⌜True⌝⦄ fib_impl n ⦃⇓ r => r = fib_spec n⦄ :
 
 #check fib_impl.fun_cases
 theorem fib_triple_cases : ⦃⌜True⌝⦄ fib_impl n ⦃⇓ r => r = fib_spec n⦄ := by
-  mintro -
   apply fib_impl.fun_cases _ ?case1 ?case2 n
-  case case1 => unfold fib_impl; mwp
+  case case1 => unfold fib_impl; mintro -; mwp
   case case2 =>
   intro n h
   unfold fib_impl
+  mintro -
   simp only [h, reduceIte]
   mwp
   mspec Specs.forIn_list (⇓ (⟨a, b⟩, xs) => a = fib_spec xs.rpref.length ∧ b = fib_spec (xs.rpref.length + 1)) ?step
   case step => dsimp; intros; mintro _; mwp; simp_all
   simp_all [Nat.sub_one_add_one]
 
-theorem fib_impl_cases
+theorem fib_impl_vcs
     (Q : Nat → PostCond Nat PostShape.pure)
-    (case1 : (Q 0).1 0)
-    (case2 : ∀ n (_ : ¬n = 0),
-             let xs := List.range' 1 (n - 1) 1
-             ∃ (I : PostCond (MProd Nat Nat × List.Zipper xs) PostShape.pure),
-               I.1 (⟨0, 1⟩, List.Zipper.begin xs)
-               ∧ (∀ r, I.1 (r, List.Zipper.end xs) ⊢ₛ (Q n).1 r.snd)
-               ∧ (∀ r rpref x suff (h : xs = rpref.reverse ++ x :: suff),
-                  I.1 (r, ⟨rpref, x::suff, by simp[h]⟩) ⊢ₛ I.1 (⟨r.2, r.1+r.2⟩, ⟨x::rpref, suff, by simp[h]⟩)))
+    (I : (n : Nat) → (_ : ¬n = 0) →
+      PostCond (MProd Nat Nat × List.Zipper (List.range' 1 (n - 1) 1)) PostShape.pure)
+    (ret : (Q 0).1 0)
+    (loop_pre : ∀ n (hn : ¬n = 0), (I n hn).1 (⟨0, 1⟩, List.Zipper.begin _))
+    (loop_post : ∀ n (hn : ¬n = 0) r, (I n hn).1 (r, List.Zipper.end _) ⊢ₛ (Q n).1 r.snd)
+    (loop_step : ∀ n (hn : ¬n = 0) r rpref x suff (h : List.range' 1 (n - 1) 1 = rpref.reverse ++ x :: suff),
+                  (I n hn).1 (r, ⟨rpref, x::suff, by simp[h]⟩) ⊢ₛ (I n hn).1 (⟨r.2, r.1+r.2⟩, ⟨x::rpref, suff, by simp[h]⟩))
     : wp⟦fib_impl n⟧.apply (Q n) := by
   apply fib_impl.fun_cases _ ?case1 ?case2 n
-  case case1 => unfold fib_impl; mstart; mwp; mpure_intro; exact case1
+  case case1 => unfold fib_impl; mstart; mwp; mpure_intro; exact ret
   case case2 =>
-  intro n h
+  intro n hn
   unfold fib_impl
   simp only [*, reduceIte]
   mstart
   mwp
-  have ⟨I, hpre, hpost, hstep⟩ := case2 n h
-  mspec Specs.forIn_list
-  case post.success => exact hpost r
+  mspec -- Specs.forIn_list
+  case pre => mpure_intro; exact loop_pre n hn
+  case post.success => exact loop_post n hn r
   case step =>
-    intro _ _ _ _ h
-    mintro _
-    mwp
-    exact hstep _ _ _ _ h
+    intro _ _ _ _ h;
+    mintro _;
+    mwp;
+    exact loop_step n hn _ _ _ _ h
 
 theorem fib_triple_cases' : ⦃⌜True⌝⦄ fib_impl n ⦃⇓ r => r = fib_spec n⦄ := by
   intro _
-  apply fib_impl_cases
-  case case1 => rfl
-  case case2 =>
-  intro n xs
-  refine ⟨(⇓ (⟨a, b⟩, xs) => a = fib_spec xs.rpref.length ∧ b = fib_spec (xs.rpref.length + 1)), ?pre, ?post, ?step⟩
-  case pre => trivial
-  case post => simp_all[Nat.sub_one_add_one]
-  case step => simp_all
+  apply fib_impl_vcs
+  case I => intro n hn; exact (⇓ (⟨a, b⟩, xs) => a = fib_spec xs.rpref.length ∧ b = fib_spec (xs.rpref.length + 1))
+  case ret => rfl
+  case loop_pre => intros; trivial
+  case loop_post => simp_all[Nat.sub_one_add_one]
+  case loop_step => simp_all
 
 theorem fib_correct {n} : (fib_impl n).run = fib_spec n := by
   generalize h : (fib_impl n).run = x
